verif/btrees/verif_splitnode_part4.v
@@ -26,7 +26,7 @@ Lemma splitnode_main_if_else_proof:
   (LEAFENTRY : LeafEntry e = LeafNode (btnode val ptr0 le isLeaf First Last nval))
   (keyrepr : val) (coprepr : val + val)
   (HEVR : entry_val_rep e = (keyrepr, coprepr))
-  (k : key) (HK : keyrepr = key_repr k)
+  (k : key) (HK : keyrepr = Vptrofs k)
   (INRANGE : 0 <= findRecordIndex n k <= Fanout)
   (vnewnode : val)
   (H1 : vnewnode <> nullval)
@@ -78,7 +78,7 @@ semax (func_tycontext f_splitnode Vprog Gprog [])
            (splitnode_right
               (btnode val ptr0 le isLeaf First Last nval) e newx);
          data_at Ews tentry
-           (key_repr
+           (Vptrofs
               (splitnode_key
                  (btnode val ptr0 le isLeaf First Last nval) e),
            inl newx) pe))%assert) (stackframe_of f_splitnode)).
@@ -175,7 +175,7 @@ Proof.
       rewrite HZNTH. simpl. auto. }
     Intros allent_end.
     forward.                    (* t'24=entry->key *)
-    rewrite HK. unfold key_repr.
+    rewrite HK.
 
     assert(FRIRANGE: 0 <= fri <= Fanout) by assumption.
     rewrite ENTRY in HEVR. simpl in HEVR. inv HEVR.
@@ -262,7 +262,7 @@ Proof.
       (* rewrite upd_Znth_app2. *)
       rewrite upd_Znth_same.
     set (fri := findRecordIndex n k) in *.
-      assert((upd_Znth (i + 1) (map entry_val_rep (sublist 0 fri le)  ++ (Vptrofs (Ptrofs.repr (k_ k)), inl (getval ce)) :: map entry_val_rep (sublist fri i le) ++ x) (key_repr ki, inl (getval ci))) 
+      assert((upd_Znth (i + 1) (map entry_val_rep (sublist 0 fri le)  ++ (Vptrofs (Ptrofs.repr (k_ k)), inl (getval ce)) :: map entry_val_rep (sublist fri i le) ++ x) (Vptrofs ki, inl (getval ci))) 
                  = (map entry_val_rep (sublist 0 fri le)  ++ (Vptrofs (Ptrofs.repr (k_ k)), inl (getval ce)) :: map entry_val_rep (sublist fri (i + 1) le) ++ sublist 1 (Zlength x) x)).
       { autorewrite with sublist. f_equal.
         change (?A::?B) with ([A]++B).
@@ -278,6 +278,7 @@ Proof.
         rewrite Znth_map in H2 by list_solve. inv H2. rewrite H3. reflexivity.
       }
       rewrite <- ?Vptrofs_repr_Vlong_repr by auto.
+    change (Vlong (Ptrofs.to_int64 ki)) with (Vptrofs ki) in *.
       rewrite H18. simpl. cancel.
       list_solve.
       list_solve.
